\documentclass[12pt]{article}%
\usepackage{amsfonts}
\usepackage{fancyhdr}
\usepackage{comment}
\usepackage[a4paper, top=2.5cm, bottom=2.5cm, left=2.2cm, right=2.2cm]%
{geometry}
\usepackage{times}
\usepackage{amsmath}
\usepackage{changepage}
\usepackage{stfloats}
\usepackage{amssymb}
\usepackage{graphicx}
\usepackage{indentfirst}
\setlength{\parindent}{2em}
\setcounter{MaxMatrixCols}{30}
\newtheorem{theorem}{Theorem}
\newtheorem{acknowledgement}[theorem]{Acknowledgement}
\newtheorem{algorithm}[theorem]{Algorithm}
\newtheorem{axiom}{Axiom}
\newtheorem{case}[theorem]{Case}
\newtheorem{claim}[theorem]{Claim}
\newtheorem{conclusion}[theorem]{Conclusion}
\newtheorem{condition}[theorem]{Condition}
\newtheorem{conjecture}[theorem]{Conjecture}
\newtheorem{corollary}[theorem]{Corollary}
\newtheorem{criterion}[theorem]{Criterion}
\newtheorem{definition}[theorem]{Definition}
\newtheorem{example}[theorem]{Example}
\newtheorem{exercise}[theorem]{Exercise}
\newtheorem{lemma}[theorem]{Lemma}
\newtheorem{notation}[theorem]{Notation}
\newtheorem{problem}[theorem]{Problem}
\newtheorem{proposition}[theorem]{Proposition}
\newtheorem{remark}[theorem]{Remark}
\newtheorem{solution}[theorem]{Solution}
\newtheorem{summary}[theorem]{Summary}
\newenvironment{proof}[1][Proof]{\textbf{#1.} }{\ \rule{0.5em}{0.5em}}

\usepackage{mathtools}

\newcommand{\Q}{\mathbb{Q}}
\newcommand{\R}{\mathbb{R}}
\newcommand{\C}{\mathbb{C}}
\newcommand{\Z}{\mathbb{Z}}

\begin{document}

\title{STAT3003 Problem Sheet 1}
\author{ZHENG Weijia (William, 1155124322)}
\date{\today}
\maketitle



\section{Q1}

We want to prove $E[\hat{\sigma}^2]=\frac{N}{N-1}\sigma^2.$

Note that $\sigma^2=\frac{1}{N}\sum_{j=1}^{N}(u_j-\mu)=\frac{1}{N^2}[(N-1)\sum_{j=1}^{N}u_j^2-\sum_{j=1}^{N}\sum_{k\neq j}u_ju_k]$

Hence R.H.S.=$\frac{N}{N-1}\sigma^2=\frac{1}{N(N-1)}[\sum_{j=1}^{N}\sum_{k\neq j}u_j^2-\sum_{j=1}^{N}\sum_{k\neq j}u_ju_k].$

Also note that $\hat{\sigma}^2=\frac{1}{n-1}\sum_{i=1}^{n}(Y_i-\bar{Y})^2=\frac{1}{n(n-1)}[(n-1)\sum_{i=1}^{n}Y_i^2-\sum_{j=1}^{n}\sum_{k\neq j}Y_jY_k]$

$=\frac{1}{n(n-1)}[(n-1)\sum_{i=1}^{n}u_i^2Z_i^2-\sum_{j=1}^{n}\sum_{k\neq j}u_ju_kZ_jZ_k].$

Hence L.H.S.=$E[\hat{\sigma}^2]=\frac{1}{n}\sum_{i=1}^{n}u_i^2E[Z_i^2]-\frac{1}{n(n-1)}\sum_{j=1}^{n}\sum_{k\neq j}u_ju_kE[Z_jZ_k]$

$=\frac{1}{n}\sum_{i=1}^{n}u_i^2E[Z_i^2]-\frac{1}{n(n-1)}\sum_{j=1}^{n}\sum_{k\neq j}u_ju_kE[Z_jZ_k]$

$=\frac{1}{n}\sum_{i=1}^{n}u_i^2\frac{n}{N}-\frac{1}{n(n-1)}\sum_{j=1}^{n}\sum_{k\neq j}u_ju_k\frac{n(n-1)}{N(N-1)}$

$=\frac{1}{N}\sum_{i=1}^{n}u_i^2-\sum_{j=1}^{n}\sum_{k\neq j}u_ju_k\frac{1}{N(N-1)}=\frac{1}{N(N-1)}[\sum_{j=1}^{N}\sum_{k\neq j}u_j^2-\sum_{j=1}^{N}\sum_{k\neq j}u_ju_k]$=R.H.S..

Q.E.D.

~\ 

\section{Q2}




\end{document}
